WIP

src/Rewriter/PerfTesting/Core.v
@@ -2,6 +2,10 @@ Require Export Coq.ZArith.ZArith.
 Require Import Coq.QArith.QArith_base Coq.QArith.Qround.
 Require Export Coq.Strings.String.
 Require Import Coq.Lists.List.
+Require Crypto.Arithmetic.Core.
+Require Crypto.Arithmetic.ModOps.
+Require Crypto.Arithmetic.Saturated.
+Require Crypto.Arithmetic.WordByWordMontgomery.
 Require Crypto.ArithmeticCPS.Core.
 Require Crypto.ArithmeticCPS.ModOps.
 Require Crypto.ArithmeticCPS.Saturated.
@@ -96,6 +100,212 @@ Module Import UnsaturatedSolinas.
                             (firstn 2 (get_possible_limbs sv cv bitwidth))
        | None => nil
        end.
+
+
+  Section foo.
+    Definition ps := Eval vm_compute in of_string "2^9-1"%string 16.
+    Definition p : params := Eval vm_compute in match ps as ps' return match ps' with nil => _ | _ => _ end with cons x _ => x | _ => I end.
+    Existing Instance p.
+    Print p.
+
+    Lemma Z_of_nat_O : Z.of_nat 0 = 0. Proof. reflexivity. Qed.
+    Hint Rewrite Z_of_nat_O : mydb.
+    Lemma Z_of_nat_S : forall x, Z.of_nat (S x) = Z.pos (Pos.of_succ_nat x). Proof. reflexivity. Qed.
+    Hint Rewrite Z_of_nat_S : mydb.
+    Hint Rewrite @Prod.fst_pair @Prod.snd_pair : mydb.
+    Lemma Z_mul_pos_pos x y : Z.pos x * Z.pos y = Z.pos (x * y). Proof. reflexivity. Qed.
+    Hint Rewrite Z_mul_pos_pos : mydb.
+    Hint Rewrite Z.mul_0_l Z.mul_0_r Z.opp_0 : mydb.
+    Lemma Z_div_0_l_pos x : 0 / Z.pos x = 0. Proof. reflexivity. Qed.
+    Hint Rewrite Z_div_0_l_pos : mydb.
+    Lemma Z_opp_pos x : Z.opp (Z.pos x) = Z.neg x. Proof. reflexivity. Qed.
+    Hint Rewrite Z_opp_pos : mydb.
+    Lemma Z_opp_neg x : Z.opp (Z.neg x) = Z.pos x. Proof. reflexivity. Qed.
+    Hint Rewrite Z_opp_neg : mydb.
+    Definition Z_div_unfolded := Eval cbv in Z.div.
+    Lemma unfold_Z_div_pos_pos x y : Z.div (Z.pos x) (Z.pos y) = Z_div_unfolded (Z.pos x) (Z.pos y).
+    Proof. reflexivity. Qed.
+    Lemma unfold_Z_div_pos_neg x y : Z.div (Z.pos x) (Z.neg y) = Z_div_unfolded (Z.pos x) (Z.neg y).
+    Proof. reflexivity. Qed.
+    Lemma unfold_Z_div_neg_pos x y : Z.div (Z.neg x) (Z.pos y) = Z_div_unfolded (Z.neg x) (Z.pos y).
+    Proof. reflexivity. Qed.
+    Lemma unfold_Z_div_neg_neg x y : Z.div (Z.neg x) (Z.neg y) = Z_div_unfolded (Z.neg x) (Z.neg y).
+    Proof. reflexivity. Qed.
+    Hint Rewrite unfold_Z_div_neg_neg unfold_Z_div_neg_pos unfold_Z_div_pos_neg unfold_Z_div_pos_pos : mydb.
+    Hint Rewrite Z.pow_0_r : mydb.
+    Definition Z_pow_unfolded := Eval cbv in Z.pow.
+    Lemma Z_pow_pos_pos x y : Z.pow (Z.pos x) (Z.pos y) = Z_pow_unfolded (Z.pos x) (Z.pos y). Proof. reflexivity. Qed.
+    Hint Rewrite Z_pow_pos_pos : mydb.
+    Lemma app_cons A (x : A) xs ys : (x :: xs) ++ ys = x :: (xs ++ ys).
+    Proof. reflexivity. Qed.
+    Hint Rewrite app_cons : mydb.
+    Lemma app_nil A xs : @nil A ++ xs = xs.
+    Proof. reflexivity. Qed.
+    Hint Rewrite app_nil : mydb.
+    Lemma partition_cons A f x xs : @partition A f (x :: xs) = prod_rect (fun _ => _) (fun g d => if f x then (x :: g, d) else (g, x :: d)) (partition f xs).
+    Proof. reflexivity. Qed.
+    Hint Rewrite partition_cons : mydb.
+    Lemma partition_nil A f : @partition A f nil = (nil, nil). Proof. reflexivity. Qed.
+    Hint Rewrite partition_nil : mydb.
+    Lemma prod_rect_pair A B P f x y : @prod_rect A B P f (x, y) = f x y. Proof. reflexivity. Qed.
+    Hint Rewrite prod_rect_pair : mydb.
+    Definition Z_modulo_unfolded := Eval cbv in Z.modulo.
+    Lemma Z_modulo_pos_pos x y : Z.modulo (Z.pos x) (Z.pos y) = Z_modulo_unfolded (Z.pos x) (Z.pos y).
+    Proof. reflexivity. Qed.
+    Hint Rewrite Z_modulo_pos_pos : mydb.
+    Hint Rewrite Z.eqb_refl Nat.eqb_refl : mydb.
+    Definition Pos_eqb_unfolded := Eval cbv in Pos.eqb.
+    Lemma Z_eqb_pos_pos x y : Z.eqb (Z.pos x) (Z.pos y) = Pos_eqb_unfolded x y. Proof. reflexivity. Qed.
+    Hint Rewrite Z_eqb_pos_pos : mydb.
+    Lemma Z_eqb_neg_neg x y : Z.eqb (Z.neg x) (Z.neg y) = Pos_eqb_unfolded x y. Proof. reflexivity. Qed.
+    Hint Rewrite Z_eqb_neg_neg : mydb.
+    Lemma Z_eqb_pos_0 x : Z.eqb (Z.pos x) 0 = false. Proof. reflexivity. Qed.
+    Hint Rewrite Z_eqb_pos_0 : mydb.
+    Lemma Z_eqb_0_pos x : Z.eqb 0 (Z.pos x) = false. Proof. reflexivity. Qed.
+    Hint Rewrite Z_eqb_0_pos : mydb.
+    Lemma Z_eqb_pos_neg x y : Z.eqb (Z.pos x) (Z.neg y) = false. Proof. reflexivity. Qed.
+    Hint Rewrite Z_eqb_pos_neg : mydb.
+    Lemma Z_eqb_neg_pos y x : Z.eqb (Z.neg y) (Z.pos x) = false. Proof. reflexivity. Qed.
+    Hint Rewrite Z_eqb_neg_pos : mydb.
+    Lemma Z_eqb_neg_0 x : Z.eqb (Z.neg x) 0 = false. Proof. reflexivity. Qed.
+    Hint Rewrite Z_eqb_neg_0 : mydb.
+    Lemma Z_eqb_0_neg x : Z.eqb 0 (Z.neg x) = false. Proof. reflexivity. Qed.
+    Hint Rewrite Z_eqb_0_neg : mydb.
+    Lemma length_nil A : List.length (@nil A) = 0%nat. Proof. reflexivity. Qed.
+    Hint Rewrite map_cons map_nil @length_cons length_nil : mydb.
+    Hint Rewrite @flat_map_cons @flat_map_nil : mydb.
+    Lemma nat_eqb_S_O x : Nat.eqb (S x) O = false. Proof. reflexivity. Qed.
+    Hint Rewrite nat_eqb_S_O : mydb.
+    Lemma nat_eqb_O_S x : Nat.eqb O (S x) = false. Proof. reflexivity. Qed.
+    Hint Rewrite nat_eqb_O_S : mydb.
+    Hint Rewrite @fold_right_cons @fold_right_nil : mydb.
+    Import Rewriter.Util.LetIn.
+    Lemma dlet_pair A B T x y f : Let_In (@pair A B x y) f = (dlet x' := x in dlet y' := y in f (x', y')) :> T.
+    Proof. reflexivity. Qed.
+    Hint Rewrite dlet_pair : mydb.
+    Lemma lift_dlet A B C x (f : A -> B) (g : B -> C) : g (Let_In x f) = Let_In x (fun x' => g (f x)). Proof. reflexivity. Qed.
+    Hint Rewrite lift_dlet : mydb.
+    Lemma inline_dlet_S B x (f : nat -> B) : Let_In (S x) f = f (S x). Proof. reflexivity. Qed.
+    Hint Rewrite inline_dlet_S : mydb.
+    Lemma inline_dlet_O B (f : nat -> B) : Let_In O f = f O. Proof. reflexivity. Qed.
+    Hint Rewrite inline_dlet_O : mydb.
+    Lemma rev_nil A : rev (@nil A) = nil. Proof. reflexivity. Qed.
+    Hint Rewrite @rev_cons @rev_nil : mydb.
+    Hint Rewrite @update_nth_nil @update_nth_cons : mydb.
+    Lemma update_nth_S_cons T n f x xs : @update_nth T (S n) f (x :: xs) = x :: update_nth n f xs.
+    Proof. reflexivity. Qed.
+    Hint Rewrite update_nth_S_cons : mydb.
+    Hint Rewrite @combine_cons @combine_nil_r : mydb.
+    Lemma app_dlet A B x (f : A -> list B) ys : (Let_In x f) ++ ys = Let_In x (fun x' => f x' ++ ys).
+    Proof. reflexivity. Qed.
+    Hint Rewrite app_dlet : mydb.
+    Print Core.Associational.split.
+    Lemma split_cons s p ps : Core.Associational.split s (p :: ps) = prod_rect (fun _ => _) (fun hi lo => (lo, List.map (fun t : Z * Z => (fst t / s, snd t)) hi)) (partition (fun t : Z * Z => fst t mod s =? 0) (p :: ps)).
+    Proof.
+      cbv [Core.Associational.split prod_rect]; edestruct partition; reflexivity.
+    Qed.
+    Hint Rewrite split_cons : mydb.
+    Lemma mul_cons_cons p ps q qs : Core.Associational.mul (p :: ps) (q :: qs) = flat_map (fun t : Z * Z => List.map (fun t' : Z * Z => (fst t * fst t', snd t * snd t')) (q :: qs)) (p :: ps).
+    Proof. reflexivity. Qed.
+    Hint Rewrite mul_cons_cons : mydb.
+    Lemma mul_cons_nil p ps : Core.Associational.mul (p :: ps) nil = flat_map (fun t : Z * Z => List.map (fun t' : Z * Z => (fst t * fst t', snd t * snd t')) nil) (p :: ps).
+    Proof. reflexivity. Qed.
+    Hint Rewrite mul_cons_nil : mydb.
+    Lemma mul_nil_cons q qs : Core.Associational.mul nil (q :: qs) = flat_map (fun t : Z * Z => List.map (fun t' : Z * Z => (fst t * fst t', snd t * snd t')) (q :: qs)) nil.
+    Proof. reflexivity. Qed.
+    Hint Rewrite mul_nil_cons : mydb.
+    Lemma mul_nil_nil : Core.Associational.mul nil nil = flat_map (fun t : Z * Z => List.map (fun t' : Z * Z => (fst t * fst t', snd t * snd t')) nil) nil.
+    Proof. reflexivity. Qed.
+    Hint Rewrite mul_nil_nil : mydb.
+
+    Declare Reduction mycbv := cbv [Pos.of_succ_nat Pos.succ Pos.mul Pos.add Z_div_unfolded Z_pow_unfolded Z_modulo_unfolded Pos_eqb_unfolded].
+
+    Opaque LetIn.Let_In.
+    Hint Constants Opaque : rewrite.
+
+    Global Instance: forall A B, Proper (eq ==> eq ==> eq) (@pair A B) := _.
+    Global Instance: forall A B P, Proper (pointwise_relation _ (pointwise_relation _ eq) ==> eq ==> eq) (@prod_rect A B (fun _ => P)).
+    Proof. intros ? ? ? f g Hfg [? ?] ? ?; subst; apply Hfg. Qed.
+    Global Instance: Transitive (Basics.flip Basics.impl) := _.
+    Existing Instance pointwise_map.
+    Existing Instance fold_right_Proper.
+    Global Instance: forall A B, Proper (forall_relation (fun _ => pointwise_relation _ eq) ==> eq ==> eq ==> eq) (@fold_right A B).
+    Proof. intros ? ? f g Hfg. apply fold_right_Proper, Hfg. Qed.
+    Global Instance: forall A B x, (Proper (pointwise_relation _ eq ==> eq) (@Let_In A (fun _ => B) x)) := _.
+
+    Goal True.
+      pose (fun f g : list Z => Arithmetic.ModOps.carry_mulmod (Qnum limbwidth) (Zpos (Qden limbwidth)) s c n idxs (ListUtil.expand_list 0 f n) (ListUtil.expand_list 0 g n)) as v.
+      cbv -[ModOps.carry_mulmod ListUtil.expand_list] in v.
+      assert (forall f g, v f g = f); subst v; intros.
+      { cbv [ListUtil.expand_list ModOps.carry_mulmod ListUtil.expand_list_helper nat_rect Arithmetic.ModOps.weight Core.Positional.mulmod Core.Positional.to_associational seq List.map List.combine Core.Associational.mul flat_map].
+        Time (rewrite_strat (((topdown (hints mydb; eval mycbv));
+                                eval cbv [Core.Associational.repeat_reduce nat_rect Core.Associational.split Core.Associational.mul];
+                                ((topdown (hints mydb; eval mycbv)));
+                                eval cbv [Core.Positional.from_associational Init.Nat.pred Core.Positional.zeros repeat Core.Positional.place nat_rect Core.Positional.add_to_nth])));
+          (* COQBUG(https://github.com/coq/coq/issues/10934) *)
+          (rewrite_strat ((try repeat (topdown (hints mydb; eval mycbv)))));
+          (rewrite_strat ((try repeat (topdown (hints mydb; eval mycbv)))));
+          (rewrite_strat eval cbv [Core.Positional.chained_carries Core.Positional.carry_reduce]);
+          (rewrite_strat ((try repeat (topdown (hints mydb; eval mycbv)))));
+          (rewrite_strat eval cbv [Core.Positional.carry Core.Positional.to_associational Core.Associational.carry seq Core.Associational.carryterm Core.Positional.from_associational]);
+          (rewrite_strat ((try repeat (topdown (hints mydb; eval mycbv)))));(*.
+        Time*)
+          (rewrite_strat ((try repeat (topdown (hints mydb; eval mycbv)))));(*.
+        Time*)
+          (rewrite_strat eval cbv [Init.Nat.pred Core.Positional.zeros repeat Core.Positional.place nat_rect]);
+          (rewrite_strat ((repeat (topdown (hints mydb; eval mycbv)))));(*.
+        Time*)
+          (rewrite_strat ((repeat (topdown (hints mydb; eval mycbv)))));
+          (rewrite_strat eval cbv [Core.Positional.add_to_nth Core.Associational.reduce]);(*.
+        Set Printing Depth 1000000.
+        Typeclasses eauto := debug.
+        Time*)
+          (rewrite_strat ((repeat (topdown (hints mydb; eval mycbv)))));(*.
+        Time*)
+          (rewrite_strat ((repeat (topdown (hints mydb; eval mycbv))))).
+        Time
+        Print Core.Associational.split.
+        Time rewrite_strat eval cbv [Core.Associational.split Core.Associational.mul].
+        Time (rewrite_strat ((repeat (topdown (hints mydb; eval mycbv))))).
+        Time rewrite_strat eval cbv [Core.Associational.split Core.Associational.mul].
+        Print Core.Associational.split.
+        Time (rewrite_strat ((repeat (topdown (hints mydb; eval mycbv))))).
+        Print update_nth.
+        Lemma fold_right
+        Hint Opaque Core.Positional.chained_carries : rewrite.
+        rewrite_strat subterms lift_dlet.
+
+        rewrite_strat (repeat (topdown (hints mydb; eval mycbv))).
+        rewrite lift_dlet.
+        cbv [Core.Positional.chained_carries].
+        rewrite_strat hints mydb.
+        setoid_rewrite dlet_pair.
+        rewrite dlet_pair.
+        Check fold_right_cons.
+
+        rewrite_strat (topdown (hints mydb2; eval mycbv)).
+        Search List.map cons.
+        Time rewrite_strat topdown ((try hints mydb); eval cbv [Pos.of_succ_nat Pos.succ Pos.mul Pos.add Z_div_unfolded Z_pow_unfolded Core.Associational.repeat_reduce]).
+        cbv [Core.Associational.repeat_reduce].
+        Time rewrite_strat bottomup (hints mydb; eval cbv [Pos.of_succ_nat Pos.succ Pos.mul Pos.add Z_div_unfolded Z_pow_unfolded]).
+        Print Z.pow.
+        Check Z.pow_0_r.
+        Print Z.div.
+        Print Z.opp.
+        Set Printing Implicit.
+        Set Printing All.
+        rewrite Prod.fst_pair.
+        rewrite_strat hints mydb.
+
+
+
+    Definition GallinaAxOf (p : params) : Dyn
+    := dyn (fun f g : list Z => ModOpsAx.carry_mulmod (Qnum limbwidth) (Zpos (Qden limbwidth)) s c n idxs (RT_ExtraAx.expand_list 0 f n) (RT_ExtraAx.expand_list 0 g n)).
+
+
+Print WordByWo
+
+
 
   Definition GallinaAxOf (p : params) : Dyn
     := dyn (fun f g : list Z => ModOpsAx.carry_mulmod (Qnum limbwidth) (Zpos (Qden limbwidth)) s c n idxs (RT_ExtraAx.expand_list 0 f n) (RT_ExtraAx.expand_list 0 g n)).
